Happpy

ConsistentTerm.v
@@ -11,6 +11,9 @@ From Elo Require Import WellTypedTerm.
 Inductive consistent_term (m : mem) : tm -> Prop :=
   | ctm_unit  :                 consistent_term m <{unit           }> 
   | ctm_nat   : forall n,       consistent_term m <{nat n          }>
+  | ctm_seq   : forall t1 t2,   consistent_term m t1    ->
+                                consistent_term m t2    ->
+                                consistent_term m <{t1; t2         }> 
   | ctm_var   : forall x,       consistent_term m <{var x          }>
   | ctm_fun   : forall x Tx t,  consistent_term m t     ->
                                 consistent_term m <{fn x Tx t      }>
@@ -70,6 +73,7 @@ Local Ltac _ctm tt :=
   match goal with
   | H : consistent_term _ <{unit        }> |- _ => clear H
   | H : consistent_term _ <{nat _       }> |- _ => clear H
+  | H : consistent_term _ <{_; _        }> |- _ => tt H
   | H : consistent_term _ <{var _       }> |- _ => clear H
   | H : consistent_term _ <{fn _ _ _    }> |- _ => tt H
   | H : consistent_term _ <{call _ _    }> |- _ => tt H
