Multistep.v
@@ -3,10 +3,8 @@ From Elo Require Import Core.
 From Elo Require Import SyntacticProperties.
 From Elo Require Import TypeProperties.
 
-From Elo Require Import ConsistentRegions.
-
 (* ------------------------------------------------------------------------- *)
-(* has-invariants                                                            *)
+(* invariants                                                                *)
 (* ------------------------------------------------------------------------- *)
 
 Definition invariants m ths :=
@@ -45,6 +43,26 @@ Proof.
          eauto using creg_preservation_base.
 Qed.
 
+Theorem invariants_preservation_rstep : forall m1 m2 ths1 ths2 tid e,
+  invariants m1 ths1 ->
+  m1 / ths1 ~~~[tid, e]~~> m2 / ths2 ->
+  invariants m2 ths2.
+Proof.
+  intros * H ?. unfold invariants in *. decompose record H. clear H.
+  split; eauto using value_preservation_rstep.
+  split; eauto using vtm_preservation_rstep.
+  split; eauto using nur_preservation_rstep.
+  split; eauto using ui_preservation_rstep.
+  split; eauto using ucr_preservation_rstep.
+  split; eauto using wtt_preservation_rstep.
+  split; eauto using ctm_preservation_rstep.
+  split; eauto using mpt_preservation_rstep.
+  split; eauto using stm_preservation_rstep.
+  split; eauto using ice_preservation_rstep.
+  split; eauto using mcreg_preservation_rstep.
+         eauto using creg_preservation_rstep.
+Qed.
+
 Theorem invariants_preservation_ustep : forall m1 m2 ths1 ths2 tc,
   invariants m1 ths1 ->
   m1 / ths1 ~~[tc]~~>* m2 / ths2 ->
@@ -79,10 +97,85 @@ Proof.
   repeat (split; trivial).
 Qed.
 
+(* ------------------------------------------------------------------------- *)
+(*                                                                           *)
+(* ------------------------------------------------------------------------- *)
 
+Corollary des_forallprogram_memory : forall m ths P,
+  forall_program m ths P -> forall_memory m P.
+Proof. intros * [? ?]. assumption. Qed.
 
+Corollary des_forallprogram_threads : forall m ths P,
+  forall_program m ths P -> forall_threads ths P.
+Proof. intros * [? ?]. assumption. Qed.
 
+Ltac solve_inva_des :=
+  unfold invariants; intros * H; decompose record H; assumption.
 
+Corollary des_inva_value : forall m ths,
+  invariants m ths -> forall_memory m value.
+Proof. solve_inva_des. Qed.
+
+Corollary des_inva_vtm : forall m ths,
+  invariants m ths -> forall_program m ths (valid_term m).
+Proof. solve_inva_des. Qed.
+
+Corollary des_inva_nur : forall m ths,
+  invariants m ths -> no_uninitialized_references m ths.
+Proof. solve_inva_des. Qed.
+
+Corollary des_inva_ui : forall m ths,
+  invariants m ths -> unique_initializers m ths.
+Proof. solve_inva_des. Qed.
+
+Corollary des_inva_ucr : forall m ths,
+  invariants m ths -> unique_critical_regions m ths.
+Proof. solve_inva_des. Qed.
+
+Corollary des_inva_wtt : forall m ths,
+  invariants m ths -> forall_program m ths well_typed_term.
+Proof. solve_inva_des. Qed.
+
+Corollary des_inva_ctm : forall m ths,
+  invariants m ths -> forall_program m ths (consistent_term m).
+Proof. solve_inva_des. Qed.
+
+Corollary des_inva_mpt : forall m ths,
+  invariants m ths -> memory_pointer_types m.
+Proof. solve_inva_des. Qed.
+
+Corollary des_inva_stm : forall m ths,
+  invariants m ths -> forall_program m ths safe_term.
+Proof. solve_inva_des. Qed.
+
+Corollary des_inva_ice : forall m ths,
+  invariants m ths -> init_cr_exclusivity ths.
+Proof. solve_inva_des. Qed.
+
+Corollary des_inva_mcreg : forall m ths,
+  invariants m ths -> forall_memory_consistent_regions m.
+Proof. solve_inva_des. Qed.
+
+Corollary des_inva_creg : forall m ths,
+  invariants m ths -> forall_threads_consistent_regions m ths.
+Proof. solve_inva_des. Qed.
+
+#[export] Hint Resolve
+  des_forallprogram_memory
+  des_forallprogram_threads
+  des_inva_value
+  des_inva_vtm
+  des_inva_nur
+  des_inva_ui
+  des_inva_ucr
+  des_inva_wtt
+  des_inva_ctm
+  des_inva_mpt
+  des_inva_stm
+  des_inva_ice
+  des_inva_mcreg
+  des_inva_creg
+  : inva.
 
 (*
 Local Corollary vp_cstep_preservation : forall m m' ths ths' tid e,
@@ -129,57 +222,57 @@ Ltac solve_vp_destruction :=
   unfold valid_program; unfold forall_program;
   intros * Hvp **; decompose [and or] Hvp; trivial.
 
-Corollary des_vp_mval : forall m ths,
+Corollary des_inva_mval : forall m ths,
   valid_program m ths -> forall_memory m value.
 Proof. solve_vp_destruction. Qed.
 
-Corollary des_vp_mwtt : forall m ths,
+Corollary des_inva_mwtt : forall m ths,
   valid_program m ths -> forall_memory m well_typed_term.
 Proof. solve_vp_destruction. Qed.
 
-Corollary des_vp_wtt : forall m ths,
+Corollary des_inva_wtt : forall m ths,
   valid_program m ths -> forall_threads ths well_typed_term.
 Proof. solve_vp_destruction. Qed.
 
-Corollary des_vp_mvad : forall m ths,
+Corollary des_inva_mvad : forall m ths,
   valid_program m ths -> forall_memory m (valid_addresses m).
 Proof. solve_vp_destruction. Qed.
 
-Corollary des_vp_vad : forall m ths,
+Corollary des_inva_vad : forall m ths,
   valid_program m ths -> forall_threads ths (valid_addresses m).
 Proof. solve_vp_destruction. Qed.
 
-Corollary des_vp_mctr : forall m ths,
+Corollary des_inva_mctr : forall m ths,
   valid_program m ths -> forall_memory m (consistently_typed_references m).
 Proof. solve_vp_destruction. Qed.
 
-Corollary des_vp_ctr1 : forall m ths,
+Corollary des_inva_ctr1 : forall m ths,
   valid_program m ths -> forall_threads ths (consistently_typed_references m).
 Proof. solve_vp_destruction. Qed.
 
-Corollary des_vp_ctr2 : forall m ths,
+Corollary des_inva_ctr2 : forall m ths,
   valid_program m ths -> forall tid, consistently_typed_references m ths[tid].
 Proof. solve_vp_destruction. Qed.
 
-Corollary des_vp_mss : forall m ths,
+Corollary des_inva_mss : forall m ths,
   valid_program m ths -> forall_memory m safe_spawns.
 Proof. solve_vp_destruction. Qed.
 
-Corollary des_vp_ss : forall m ths,
+Corollary des_inva_ss : forall m ths,
   valid_program m ths -> forall_threads ths safe_spawns.
 Proof. solve_vp_destruction. Qed.
 
-Corollary des_vp_sms : forall m ths,
+Corollary des_inva_sms : forall m ths,
   valid_program m ths -> safe_memory_sharing m ths.
 Proof. solve_vp_destruction. Qed.
 
 #[export] Hint Resolve
-  des_vp_mval
-  des_vp_mwtt des_vp_wtt
-  des_vp_mvad des_vp_vad
-  des_vp_mctr des_vp_ctr1 des_vp_ctr2
-  des_vp_mss  des_vp_ss 
-  des_vp_sms
+  des_inva_mval
+  des_inva_mwtt des_inva_wtt
+  des_inva_mvad des_inva_vad
+  des_inva_mctr des_inva_ctr1 des_inva_ctr2
+  des_inva_mss  des_inva_ss 
+  des_inva_sms
   : vp.
 
 Corollary memtyp_multistep_preservation : forall m m' ths ths' ad tc,
