NoWRef.v
@@ -10,6 +10,9 @@ From Elo Require Import HasVar.
 Inductive no_wref (ad : addr) : tm -> Prop :=
   | nowref_unit  :                 no_wref ad <{unit          }>
   | nowref_nat   : forall n,       no_wref ad <{nat n         }>
+  | nowref_seq   : forall t1 t2,   no_wref ad t1 ->
+                                   no_wref ad t2 ->
+                                   no_wref ad <{t1; t2        }>
   | nowref_var   : forall x,       no_wref ad <{var x         }>
   | nowref_fun   : forall x Tx t,  no_wref ad t  ->
                                    no_wref ad <{fn x Tx t     }>
@@ -44,6 +47,7 @@ Local Ltac _nowref tt :=
   match goal with
   | H : no_wref _   <{unit        }> |- _ => clear H
   | H : no_wref _   <{nat _       }> |- _ => clear H
+  | H : no_wref _   <{_; _        }> |- _ => tt H
   | H : no_wref _   <{var _       }> |- _ => clear H
   | H : no_wref _   <{fn _ _ _    }> |- _ => tt H
   | H : no_wref _   <{call _ _    }> |- _ => tt H
@@ -95,6 +99,10 @@ Definition no_wrefs (t : tm) := forall ad, no_wref ad t.
 Local Ltac solve_inv_nowrefs :=
   unfold no_wrefs; intros; try split; intros; spec; invc_nowref; auto.
 
+Local Lemma inv_nowrefs_seq : forall t1 t2,
+  no_wrefs <{t1; t2}> -> no_wrefs t1 /\ no_wrefs t2.
+Proof. solve_inv_nowrefs. Qed.
+
 Local Lemma inv_nowrefs_fun : forall x Tx t,
   no_wrefs <{fn x Tx t}> -> no_wrefs t.
 Proof. solve_inv_nowrefs. Qed.
@@ -139,6 +147,7 @@ Ltac invc_nowrefs :=
   match goal with
   | H : no_wrefs <{unit        }> |- _ => clear H
   | H : no_wrefs <{nat _       }> |- _ => clear H
+  | H : no_wrefs <{_; _        }> |- _ => eapply inv_nowrefs_seq   in H as [? ?]
   | H : no_wrefs <{var _       }> |- _ => clear H
   | H : no_wrefs <{fn _ _ _    }> |- _ => eapply inv_nowrefs_fun   in H
   | H : no_wrefs <{call _ _    }> |- _ => eapply inv_nowrefs_call  in H as [? ?]
