TypeProperties.v
@@ -4,4 +4,5 @@ From Elo Require Export PointerTypes.
 From Elo Require Export Soundness.
 From Elo Require Export SafeTerm.
 From Elo Require Export ExclusivityInitCR.
+From Elo Require Export ConsistentRegions.
 
